\documentclass[12pt]{article}
\usepackage{HomeWorkTemplate}
\usepackage{circuitikz}
\usepackage{tikz}
\newcommand*\coin[1]{\tikz[baseline=(char.base)]{
            \node[shape=circle,draw,inner sep=2pt,minimum size=10mm] (char) {#1};}}
\usepackage{float}
\usepackage{xepersian}
\usetikzlibrary{arrows,automata}
\usetikzlibrary{circuits.logic.US}
\settextfont{B Nazanin}
\newcounter{problemcounter}
\newcounter{subproblemcounter}
\linespread{1.2}
\setcounter{problemcounter}{1}
\setcounter{subproblemcounter}{1}
\newcommand{\grade}[1]{\textbf{(#1 نمره)}}
\newcommand{\problem}[1]
{
\subsection*{
مسأله‌ی
\arabic{problemcounter} 
\stepcounter{problemcounter}
\setcounter{subproblemcounter}{1}
#1
}
}
\newcommand{\subproblem}{
\textbf{\harfi{subproblemcounter})}\stepcounter{subproblemcounter}
}
\newcommand{\n}{

\null

}
\begin{document}

\handout
{احتمال و کاربرد}
{}
{8 آبان 1398}
{سری 1}
{14 آبان}
علیرضا درویشی................................................................................................................................................................................. ۹۶۱۰۹۶۷۴
\subsection*{مسأله ۱}
الف)
\begin{flushleft}
$P(B_i | A)=\frac{P(B_i)P(A|B_i)}{\sum_{j=1}^{j=k}P(B_j)P(A|B_i)}$

$P(1st\ black | 2nd \ red)=\frac{P(1st\ black)P(2nd\ red|1st\ black)}{P(1st\ black)P(2nd\ red|1st\ black)+P(1st\ red)P(2nd\ red|1st\ red)}$

$\Rightarrow P(1st\ black | 2nd \ red)=\frac{\frac{b}{r+b}\frac{r}{r+b+c}}{\frac{b}{r+b}\frac{r}{r+b+c}+\frac{r}{r+b}\frac{r+c}{r+b+c}}=\frac{b}{r+b+c}$


\end{flushleft}
ب)
\begin{flushleft}
$for \ i\ : A_i= \{i\in A\ \& i\in B\} \parallel \{i\notin A\ \& i\in B\} \parallel \{i\notin A\ \& i\notin B\}$

$for \ i\ : p(A_i)=\frac{3}{4}$

$p(\bigcap^n_{i=1}A_i)=(\frac{3}{4})^n$
\end{flushleft}


ج)

\begin{flushleft}
$p(E|E\cup F)=\frac{p(E\cap (E\cup F))}{p(E\cup F)}\frac{p(E)}{p(E\cup F)}=\frac{p(E\cap F)+p(E\cap F^c)}{p(F)+p(E\cap F^c)}\geq \frac{p(E\cap F)}{p(F)}=p(E|F) $



\end{flushleft}

\subsection*{مسأله‌ ۲}
\begin{flushleft}
$\overbrace{\coin{$?$}\coin{$?$}\coin{$?$}....\coin{$?$}}^\text{$n$} : \coin{$H$}\coin{$T$}\overbrace{\coin{$?$}....\coin{$?$}}^\text{$n-2$}\ or\ \coin{$T$}\overbrace{\coin{$?$}\coin{$?$}....\coin{$?$}}^\text{$n-1$}$

$ $

$\Rightarrow f_n=f_{n-1}+f_{n-2}$

$f_0=1$

$f_1=2$

\end{flushleft}
\subsection*{مسأله‌ی ۳}
\begin{flushleft}
$n_A: \ number\ of \ heads\ in \ A$

$n_B: \ number\ of \ heads\ in \ B$

$p(n_A=n_B)=\sum_j p(n_A=j,n_B=j)=\sum_j p(n_A=j)p(n_B=j)=\sum_j (\frac{1}{2})^k \binom{k}{j} (\frac{1}{2})^{n-k} \binom{n-k}{j}=(\frac{1}{2})^n \sum_j \binom{k}{j}\binom{n-k}{j}=(\frac{1}{2})^n\binom{n}{k}=p(n_A+n_B=k)$
\end{flushleft}
\subsection*{مسأله‌ی ۴}
\begin{flushleft}
$p(X=x)=
\frac{n}{n+m}\frac{n-1}{n+m-1}...\frac{n-(x-1)}{n+m-(x-1)}\times\frac{m}{n+m-x}=
\frac{m}{n+m-x}\frac{\frac{n!}{(n-x)!}}{\frac{(n+m)!}{(n+m-x)!}}=
\frac{m}{n+m-x}\frac{\frac{(n+m-x)!}{(n-x)!}}{\frac{(n+m)!}{n!}}=
\frac{m}{n+m-x}\frac{\binom{n+m-x}{m}}{\binom{n+m}{m}}=
\frac{\binom{n+m-1-x}{m-1}}{\binom{n+m}{m}}$

$E[X]=\sum_{x=1}^{n} xp(X=x)=
\sum_{x=1}^{n} x \frac{\binom{n+m-1-x}{m-1}}{\binom{n+m}{m}}=
\frac{1}{\binom{n+m}{m}}\sum_{x=1}^{n} x \binom{n+m-1-x}{m-1}=
\frac{1}{\binom{n+m}{m}}\sum_{j=1}^{n} \underbrace{\sum_{x=j}^{n} \binom{n+m-1-x}{m-1}}_{\sum_{k=m}^n \binom{k}{m}=\binom{n+1}{m+1}}=
\frac{1}{\binom{n+m}{m}}\sum_{j=1}^{n} \binom{m-1+n-j+1}{m-1+1}=
\frac{1}{\binom{n+m}{m}} \underbrace{\sum_{j=1}^{n} \binom{m+n-j}{m}}_{\sum_{k=m}^n \binom{k}{m}=\binom{n+1}{m+1}}=
\frac{1}{\binom{n+m}{m}} \binom{n+m}{m+1}=\frac{\frac{(n+m)!}{(m+1)!(n-1)!}}{\frac{(n+m)!}{n!m!}}=
\boxed{\frac{n}{m+1}}$

\end{flushleft}
\subsection*{مسأله‌ ۵}
\begin{flushleft}
$f(x)=e^{-x^2/2}$

$f_1(x)=(1+\frac{1}{x^2})e^{-x^2/2}$

$f_2(x)=\frac{x^4+2x^2-1}{x^4+2x^2+1}e^{-x^2/2}$

$\Rightarrow f_2(x)\leq f(x) \leq f_1(x) \Rightarrow \int_x^{\infty}f_2(y)dy\leq\int_x^{\infty}f(y)dy\leq\int_x^{\infty}f_1(y)dy$

$\Rightarrow \frac{1}{\sqrt{2\pi}}\frac{x}{x^2+1}e^{-\frac{x^2}{2}}\leq p(Z\geq x)\leq \frac{1}{\sqrt{2\pi}}\frac{1}{x}e^{-\frac{x^2}{2}}$
\end{flushleft}
\subsection*{مسأله‌ ۶}
الف)
\begin{flushleft}
$J=
\begin{pmatrix} 
\partial x \\
\partial y
\end{pmatrix}
\begin{pmatrix} 
U & V
\end{pmatrix}
=
\begin{pmatrix} 
U_x & V_x \\
U_y & V_y
\end{pmatrix}
=
\begin{pmatrix} 
y & 1/y\\
x& -x/y^2
\end{pmatrix}
=
-2x/y=-2V
$

$g(U,V)=f(x,y)\frac{1}{|J|}=\frac{1}{2U^2V}$

$g(U,V)= \begin{cases} 
      \frac{1}{2U^2V} & 0< V\  \& \ max(V,\frac{1}{V}) \leq U \\
      0 & else
   \end{cases}
$

\end{flushleft}
ب)
\begin{flushleft}
$f_U(U)=\int_{V=\frac{1}{U}}^{U} g(U,V)dV=\frac{1}{U^2}ln(U)$

$f_V(V)=\int_{U} g(U,V)dV$

$f_V(V)=\begin{cases} 
      \int_{U=V}^{\infty} g(U,V)dU=\frac{1}{2V^2} & V\geq 1 \\
      \int_{U=\frac{1}{V}}^{\infty} g(U,V)dU=\frac{1}{2} & 0<V \leq 1
   \end{cases}$
\end{flushleft}
\subsection*{مسأله‌ ۷}
\begin{flushleft}
$E[X_1+X_2+..+X_n|X_1+X_2+..+X_n=x]=x$

$E[X_1+X_2+..+X_n|X_1+X_2+..+X_n=x]=E[X_1|X_1+X_2+..+X_n=x]+E[X_2|X_1+X_2+..+X_n=x]+..+E[X_n|X_1+X_2+..+X_n=x]=nE[X_1|X_1+X_2+..+X_n=x]$

$\Rightarrow E[X_1|X_1+X_2+..+X_n=x]=\frac{x}{n}$
\end{flushleft}
\subsection*{مسأله‌ ۸}
الف)
\begin{flushleft}
$x_i:\begin{cases} 
      1 & ith\ ball\ is\ red \\
      0 & else
   \end{cases},\ 
X=\sum_{i=1}^{12}{x_i} \ $

$y_i:\begin{cases} 
      1 & ith\ ball\ is\ blue \\
      0 & else
   \end{cases},\ 
Y=\sum_{i=1}^{12}{y_i} \ $


$Cov(X,Y)=E[XY]-E[X]E[Y]=E[\sum x_i \sum y_j]-E[\sum x_i]E[\sum y_i]$

$E[\sum x_i\sum y_i]=E[\sum x_iy_i]+E[\sum_{i\neq j}x_iy_j]=\sum \underbrace{E[x_iy_i]}_{=0}+\sum_{i\neq j}E[x_iy_j]$

$=12\times11\times E[x_i]E[y_i]$

$ Cov(X,Y)=(12\times 11-12\times 12)E[x_i]E[y_i]=-12E[x_i]E[y_i]=-12\frac{12\times10}{30}\frac{12\times8}{30}=\boxed{-153.6}$
\end{flushleft}
ب)
\begin{flushleft}
$E[XY]=\iint_{x,y}xyf(x,y)dx dy=\frac{1}{2}\int_{y=0}^{\pi/2}ydy\{\int_{x=0}^{\pi/2}xsin(x+y)dx\}=
\frac{1}{2}\int_{y=0}^{\pi/2}y\{\frac{1}{2}(\pi-2)sin(y)+cos(y)\}dy=
\frac{\pi-2}{2}$

$E[X]=\iint_{x,y}xf(x,y)dx dy=\frac{1}{2}\int_{y=0}^{\pi/2}dy\{\int_{x=0}^{\pi/2}xsin(x+y)dx\}=
\frac{1}{2}\int_{y=0}^{\pi/2}\{\frac{1}{2}(\pi-2)sin(y)+cos(y)\}dy=
\frac{\pi}{4}$

$E[X^2]=\iint_{x,y}x^2f(x,y)dx dy=\frac{1}{2}\int_{y=0}^{\pi/2}dy\{\int_{x=0}^{\pi/2}x^2sin(x+y)dx\}=
\frac{1}{8}(\pi^2+4\pi-16)$

$\sigma_x^2=E[X^2]-E^2[X]=\frac{1}{16}(\pi^2+8\pi-32)$

$Cov(X,Y)=(\frac{\pi-2}{2})-\frac{\pi^2}{16}$

$\rho(X,Y)=\frac{(\frac{\pi-2}{2})-\frac{\pi^2}{16}}{\frac{1}{16}(\pi^2+8\pi-32)}=-0.25\neq -1$

\end{flushleft}
\subsection*{مسأله ‌9}
\begin{flushleft}
$p(|X- \mu |> \epsilon)=\frac{VAR(X)}{\epsilon^2}=\frac{VAR(X)}{n\epsilon^2}=\frac{\mu (1-\mu)}{n\epsilon^2}\leq \frac{1}{4} \frac{1}{n\epsilon^2} \leq 1-\eta\Rightarrow n\geq \frac{1}{4(1-\eta)\epsilon^2}=62500$
\end{flushleft}
\end{document}
